Work on modularizing proofs and equivalence between game transformations

FraudProof/Games/Base/ElemInTree.lean
@@ -5,6 +5,11 @@ import FraudProof.DataStructures.Sequence
 
 import Mathlib.Data.Fin.Tuple.Basic
 
+----------------------------------------
+-- * Element in Tree basic game definitions Linear game and simple games playing
+-- with the idea of needing to have the element in question or not. If we do not
+-- have the element, we play games only with hashes.
+
 -- DA: element is in Tree
 structure ElemInMTree (α ℍ : Type) where
   elem : α
@@ -25,6 +30,7 @@ def mid_condition {ℍ : Type}[BEq ℍ][mag : HashMagma ℍ]
     := match p with
       | .Next ⟨hl, hr⟩ => condWProp $ mag.comb hl hr == h
 
+-- Element in Tree arbitration game! Intermediate steps
 def arbElem {α ℍ : Type}
     (pos : Skeleton)
     [BEq ℍ]
@@ -53,6 +59,7 @@ def arbElem {α ℍ : Type}
     termination_by da.path
     decreasing_by {simp_wf; rw [_HC]; simp}
 
+-- Element in Tree arbitration game!
 def arbElemInit {α ℍ : Type} [BEq ℍ] [Hash α ℍ][HashMagma ℍ]
     -- DA
     (da : ElemInMTree α ℍ)
@@ -69,33 +76,8 @@ structure ElemInTreeN (n : Nat)(α ℍ : Type) where
   -- Let |bt : BTree α| be the implicit data, such that |hash bt = mtree|.
   -- This da says |bt ! data.2| leads to |data.1|
 
-theorem ElemInTreeN0 {α ℍ : Type} (da : ElemInTreeN 0 α ℍ)
- : da.data.2 = nilSeq
- := by have ⟨ ⟨ a , sk ⟩ , mtree ⟩ := da
-       simp
-       apply funext
-       intro empty
-       simp [nilSeq]
-       have ⟨ n , e ⟩ := empty
-       simp at e
-
-structure ElemInTreeH (n : Nat)(ℍ : Type) where
-  data : ℍ × ISkeleton n
-  mtree : ℍ
-  -- Same as above but only using hashes
-  -- |dt ! data.2| leads to | data.1| where |data.1| is the hash of the element
-  -- in a tree [see the above DA].
-
 def SingleLastStep {α ℍ : Type}[BEq ℍ][h : Hash α ℍ] (data : ElemInTreeN 0 α ℍ) : Winner
   := condWProp $ h.mhash (data.data.1) == data.mtree
-
--- Same as opHash??
--- I use SkElem to signal where the path is going.
-@[simp]
-def op_side {α : Type}[mag : HashMagma α] (o : SkElem) (a b : α) : α
- := match o with
-   | .inl _ => mag.comb a b
-   | .inr _ => mag.comb b a
 
 def SingleMidStep {ℍ : Type}[BEq ℍ][m : HashMagma ℍ ](data : ℍ × ℍ × ℍ) : Winner
   := condWProp $ m.comb data.2.1 data.2.2 == data.1
@@ -128,12 +110,21 @@ def elemInHGame {α ℍ : Type}
                (tailSeq proposer)
                (tailSeq chooser)
 
+structure ElemInTreeH (n : Nat)(ℍ : Type) where
+  data : ISkeleton n -- This is the 'skeleton proof'
+  mtree : ℍ × ℍ
+  -- Same as above but only using hashes
+  -- |dt ! data| leads to | mtree.2.2 | where |mtree.2.1| is the hash of the element
+  -- in a tree [see the above DA].
+
 -- Here we can have some troubles. We do not know if we really are talking about
 -- the same element.
+-- If path is of length 0, then elements should be the same. Although, hashes
+-- are the same, elements maybe not be.
 def SingleLastStepH {ℍ : Type}[BEq ℍ] (data : ElemInTreeH 0 ℍ) : Winner
-  := condWProp $ data.data.1 == data.mtree
+  := condWProp $ data.mtree.1 == data.mtree.2
 
-def elemInHGameH {ℍ : Type}
+def elem_in_tree_backward {ℍ : Type}
     [BEq ℍ][HashMagma ℍ]
     {n : Nat}
     (da : ElemInTreeH n ℍ)
@@ -146,743 +137,47 @@ def elemInHGameH {ℍ : Type}
          match headSeq proposer with
          | .none => Player.Chooser -- Proposer forfeits the game
          | .some (.Next proposed) =>
-           match headSeq chooser ⟨ da.mtree , proposed ⟩ with
+           match headSeq chooser ⟨ da.mtree.2 , proposed ⟩ with
            | .none => Player.Proposer -- Chooser forfeits the game
-           | .some .Now => SingleMidStep  ⟨ da.mtree , proposed ⟩
+           | .some .Now => SingleMidStep  ⟨ da.mtree.2 , proposed ⟩
            | .some (.Continue _) =>
-             have nextHash := match headSeq da.data.2 with
+             have nextHash := match headSeq da.data with
                     | .inl _ => proposed.1
                     | .inr _ => proposed.2
-             elemInHGameH
+             elem_in_tree_backward
                -- Next step DA
-               ⟨⟨ da.data.1, tailSeq da.data.2⟩ , nextHash ⟩
+               { data := tailSeq da.data, mtree := ⟨ da.mtree.1 , nextHash⟩  }
                -- Next step players
                (tailSeq proposer)
                (tailSeq chooser)
 
---------------------------------------------------------------------------------
--- Transformation from a Sequence to the /same/ game played over Trees arenas.
---------------------------------------------------------------------------------
-
--- Building a Tree out of skelentons.
--- This function keeps size.
--- ABTree.size is height
-def skeleton_to_tree {n : Nat} (sk : ISkeleton n) : ABTree Unit Unit
- := match n with
-   | .zero => .leaf ()
-   | .succ _pn => match headSeq sk with
-                 | .inl _ =>
-                        .node () (skeleton_to_tree (Fin.tail sk)) (.leaf ())
-                 | .inr _ =>
-                        .node ()  (.leaf ()) (skeleton_to_tree (Fin.tail sk))
-
 @[simp]
-def skl_to_maybe_elem {α : Type} {n : Nat}
-  (a : α) (sk : ISkeleton n) : ABTree (Option α) Unit
-    := match n with
-    | .zero => .leaf a
-    | .succ _pn => match headSeq sk with
-                    | .inl _ =>
-                            .node () (skl_to_maybe_elem a (Fin.tail sk)) (.leaf none)
-                    | .inr _ =>
-                            .node () (.leaf none) (skl_to_maybe_elem a (Fin.tail sk))
+def forward_mid_step_condition {ℍ : Type}[BEq ℍ][m : HashMagma ℍ ]
+  (side : SkElem) (data : ℍ × ℍ) (res : ℍ) : Winner
+  := condWProp $ op_side side data.1 data.2 == res
 
-@[simp]
-def build_proposer {ℍ : Type}{n : Nat}
-  (data : ℍ × ISkeleton n) (rev : Sequence n (Option (PMoves ℍ)))
-  : ABTree (Option ℍ) (Option (Unit × ℍ × ℍ))
-  := match n with
-  | .zero => .leaf <| .some data.1
-  | .succ _pn => let rest_tree := build_proposer ⟨ data.1 , Fin.tail data.2⟩ (Fin.tail rev)
-     match headSeq rev with
-       | .none => .node .none rest_tree (.leaf .none)
-       | .some (.Next ⟨ hl , hr⟩)=>
-         match headSeq data.2 with
-         | .inl _ =>
-           .node (.some ⟨ (), hl, hr ⟩)
-                 rest_tree
-                 (.leaf (.some hr))
-         | .inr _ =>
-           .node (.some ⟨ (), hl, hr ⟩)
-                 (.leaf (.some hl))
-                 rest_tree
-@[simp]
-def build_chooser {ℍ : Type}{n : Nat}
-  (data : ℍ × ISkeleton n)
-  (chooser : Sequence n (ℍ × ℍ × ℍ -> Option ChooserSmp))
-  : ABTree Unit (ℍ × Unit × ℍ × ℍ -> Option ChooserMoves)
-  := match n with
-    | .zero => .leaf ()
-    | .succ _pn =>
-      let side_choose (s : Chooser.Side) (arg : ℍ × Unit × ℍ × ℍ) : Option ChooserMoves :=
-          have ⟨ ht , _ , hl , hr ⟩ := arg
-          (headSeq chooser ⟨ ht, hl , hr ⟩).map
-            (fun ch => match ch with
-                       | .Now => .Now
-                       | .Continue _ => .Continue s)
-      match headSeq data.2 with
-      | .inl _ =>
-        .node
-          (side_choose .Left)
-          (build_chooser ⟨data.1 , Fin.tail data.2⟩ (Fin.tail chooser))
-          (.leaf ())
-      | .inr _ =>
-        .node
-          (side_choose .Right)
-          (.leaf ())
-          (build_chooser ⟨data.1 , Fin.tail data.2⟩ (Fin.tail chooser))
-
-def elem_in_tree_gen_tree {ℍ : Type}
-    [BEq ℍ][mag : HashMagma ℍ]
-    -- DA
+-- Reverse game -- It is not (*JUST*) the reverse game.
+-- Proposer proposes different hashes that the previos linear game.
+--
+def elem_in_tree_forward {ℍ : Type}[BEq ℍ][HashMagma ℍ]
     {n : Nat}
     (da : ElemInTreeH n ℍ)
-    --
     (proposer : Sequence n (Option (PMoves ℍ)))
     (chooser : Sequence n (ℍ × ℍ × ℍ -> Option ChooserSmp))
-    --
     : Winner
-    :=
-    let da_tree : CompTree (Option ℍ) Unit ℍ := {data := skl_to_maybe_elem da.data.1 da.data.2 , res := da.mtree}
-    let tree_revealer : ABTree (Option ℍ) (Option (Unit × ℍ × ℍ))
-      := build_proposer da.data proposer
-    let tree_chooser : ABTree Unit (ℍ × Unit × ℍ × ℍ -> Option ChooserMoves)
-      := build_chooser da.data chooser
-    treeCompArbGame
-      (fun opth _h1 h2 =>
-        match opth with
-        | .none => -- this case is a bit artificial
-        -- chooser should challenge previous step.
-          Player.Proposer
-        | .some hp => condWProp <| (hp == h2)
-      )
-      (fun _ _ hres pl pr =>
-        -- _nodeh and hres should be the same.
-           condWProp $ mag.comb pl pr == hres)
-      da_tree tree_revealer tree_chooser
-
-----------------------------------------
--- Are both games equivs?
---
---Two games (in this case) are equivalente if they have the same outcome to the
---same players.
-
-theorem seq_equiv_tree {ℍ : Type}[BEq ℍ][HashMagma ℍ]
-  -- DA
-  {n : Nat}(da : ElemInTreeH n ℍ)
-  -- Players
-  (proposer : Sequence n (Option (PMoves ℍ)))
-  (chooser : Sequence n (ℍ × ℍ × ℍ -> Option ChooserSmp))
-  : elemInHGameH da proposer chooser = elem_in_tree_gen_tree da proposer chooser
-  := by revert n
-        intro n
-        induction n with
-        | zero =>
-          intros da prop cho
-          simp [elemInHGameH , elem_in_tree_gen_tree, SingleLastStepH, treeCompArbGame]
-        | succ pn HInd =>
-          intros da prop cho
-          simp [elemInHGameH, elem_in_tree_gen_tree ]
-          cases prop 0 with
-          | none =>
-            simp [treeCompArbGame]
-          | some proposed =>
-            cases proposed with
-            | End v => contradiction
-            | Next e =>
-              simp
-              match HCho : cho 0 (da.mtree, e) with
-              | none =>
-                simp [treeCompArbGame]
-                match da.data.2 0 with
-                | .inl _ => simp [treeCompArbGame]; rw [HCho]; simp
-                | .inr _ => simp [treeCompArbGame]; rw [HCho]; simp
-              | some choosed =>
-                match choosed with
-                | .Now =>
-                  simp [SingleMidStep]
-                  cases da.data.2 0 with
-                    | inl _ => simp [treeCompArbGame]; rw [HCho]; simp
-                    | inr _ => simp [treeCompArbGame]; rw [HCho]; simp
-                | .Continue _ =>
-                  simp
-                  cases da.data.2 0 with
-                    | inl _ =>
-                      simp [treeCompArbGame]
-                      rw [HCho]; simp
-                      apply HInd
-                    | inr _ =>
-                      simp [treeCompArbGame]
-                      rw [HCho]; simp
-                      apply HInd
-----------------------------------------
-
-
-----------------------------------------
--- Logarithmic Search Definitions
--- It should be vector, but I wanna keep the other.
-
--- def iskehash {ℍ : Type} {n : Nat}
---   (side_skeleton : ISkeleton n)
---   (rev : Sequence n (Option (PMoves ℍ)))
---   : Sequence n (Option (Sum ℍ ℍ))
---   := seq_zip_with
---      (fun sk opt_moves =>
---      match sk with
---      | .inl _ => opt_moves.map ( .inl ∘ fun x => match x with | .Next p => p.1)
---      | .inr _ => opt_moves.map ( .inr ∘ fun x => match x with | .Next p => p.2)
---      )
---      side_skeleton rev
-
--- abbrev Side (ℍ : Type) := Sum ℍ ℍ
--- def build_log_proposer {ℍ : Type}{lgn : Nat}
---   (rev : Sequence (2^lgn.succ - 1) (Option (Side ℍ)))
---   : ABTree (Option (Side ℍ)) (Option (Side ℍ))
---   := perfectSeq rev
-
--- def from_side {α : Type} (sa : Side α) : α :=
---   match sa with
---   | .inl a => a
---   | .inr a => a
-
--- Macro to make everything shorter.
--- @[simp]
--- def Range (α : Type) := α × α
-
-structure DA_Statement (ℍ : Type) where
-  src : ℍ
-  dst : ℍ
-  len : Nat
-
---
-@[simp]
-def Tree_Reveler (ℍ : Type)
-  := ABTree (Option ℍ) (Option (Unit × DA_Statement ℍ × DA_Statement ℍ))
-
-@[simp]
-def Tree_Reveler.top {ℍ : Type} : Tree_Reveler ℍ -> Option ℍ
-  | .leaf oh => oh
-  | .node (.some ⟨ _, ⟨ _, hmid , _⟩ , _ ⟩ ) _ _ => .some hmid
-  | _ => .none
--- Good DAs also have some stuff like
--- da.len = 0 => da.src = da.dst
--- They form a metric space, topology and stuff
-
-@[simp]
-def Tree_DA (ℍ : Type) :=
-  CompTree
-    Unit -- No info at leaves
-    Unit -- No info at nodes
-    (DA_Statement ℍ) -- [a, b] and length ...
-
-@[simp]
-def all_true (ls : List Bool) : Bool := ls.all id
-
-def leaf_condition_transformation {ℍ : Type}[BEq ℍ]
-  : Unit -> ℍ -> DA_Statement ℍ-> Winner
-  := (fun _ prop ⟨ src , dst , len ⟩
-    -- Unitary range and proposed same hash
-    -- This is the end of the game. If nothing happened before.
-     => condWProp $ all_true
-     -- Unitary range [prop,prop] of length 0
-     [ len == 0
-     , prop == src
-     , src == dst
-     ]
-     )
-
-def mid_condition_transformation{ℍ : Type}[BEq ℍ][mag : HashMagma ℍ]
-  -- Arena conditions
-  : Unit -> Unit
-  -> DA_Statement ℍ -> DA_Statement ℍ -> DA_Statement ℍ
-  -> Winner
-  := (fun _ _
-        hres hl hr =>
-        let ⟨ parent_from , parent_to, len ⟩ := hres
-        let ⟨ left_from , left_to, left_len ⟩ := hl
-        let ⟨ right_from , right_to, right_len ⟩ := hr
-          -- Mid condition is the expected one
-        condWProp $
-          all_true
-          -- Path consistency
-          [ parent_from == left_from
-          , parent_to == right_to
-          , left_to == right_from
-          , left_len + right_len == len
-          , left_len > 0
-          , right_len > 0
-          -- Last condition (before leaf)
-          , (not (len == 2))
-            || (mag.comb parent_from parent_to == left_to)
-          ]
-      )
-
-def element_in_tree_transform {ℍ : Type}[BEq ℍ][m : HashMagma ℍ]
-    --
-    -- Da is a computation arena plus a range
-    -- Given |[hl, hr]| you play the arena to prove that there is a path
-    -- from |h_l| to |h_r| of length |len| (DA_Statement)
-    (da : CompTree Unit Unit (DA_Statement ℍ))
-    --
-    (proposer : ABTree (Option ℍ)
-                       (Option (Unit × (DA_Statement ℍ) × (DA_Statement ℍ))))
-    (chooser : ABTree Unit
-                      (DA_Statement ℍ × Unit × (DA_Statement ℍ) × (DA_Statement ℍ)
-                      -> Option ChooserMoves))
-    --
-    :=
-    treeCompArbGame
-      leaf_condition_transformation
-      mid_condition_transformation
-      da proposer chooser
-
--- @[simp]
--- def total_range_tree {ℍ : Type}
---   : (ABTree ℍ (Range ℍ × Range ℍ)) -> Range ℍ
---   | .leaf h => ⟨ h , h ⟩
---   | .node ⟨ left_range , right_range ⟩ _ _ => ⟨ left_range.1, right_range.2 ⟩
-
--- @[simp]
--- def get_total_range_tree {ℍ : Type}
---   (tree : ABTree (Option ℍ) (Option (Unit × (Range ℍ) × (Range ℍ))))
---   : Option (Range ℍ)
---   := match tree with
---   | .leaf (.some h) => .some ⟨ h , h ⟩
---   | .node (.some ⟨_, left_range , right_range ⟩) _ _ =>
---     .some $ ⟨ left_range.1 , right_range.2 ⟩
---   | _ => .none
-
--- Proposer transformatino
--- def logarithmic_proposer {ℍ : Type}{mag : HashMagma ℍ}{lgn : Nat}
---   (sides : ISkeleton (2^lgn.succ - 1))
---   (proposer : Sequence (2^lgn.succ - 1) (Option (PMoves ℍ)))
---   : ABTree (Option ℍ) (Option (Unit × (Range ℍ) × (Range ℍ)))
---   := match lgn with
---      | .zero =>
---        .leaf $
---          (headSeq proposer).map
---             (fun (.Next ⟨hl , hr⟩)
---               => -- We return the sibiling hash!
---                 match headSeq sides with
---                  | .inl _ => hr
---                  | .inr _ => hl
---               -- h_extra -- @op_side ℍ mag (headSeq sides) h_bot h_extra
---               )
---             -- TODO add Unit range -> true
---             -- let h_top := @op_side ℍ mag (headSeq sides) h_bot h_extra
---             -- .node (.some ⟨ (), ⟨ h_bot , h_bot⟩ , ⟨ h_top , h_top ⟩ ⟩)
---             --       -- Leafs are winning positions for the proposer.
---             --       (.leaf $ .some h_bot)
---             --       (.leaf $ .some h_top)
---      | .succ _pn =>
---        -- Sides path info
---        let ⟨ sides_left, sides_mid , sides_right ⟩ := seqPerfectSplit sides
---        -- Reveler data
---        let ⟨ prop_left, prop_mid, prop_right ⟩ := seqPerfectSplit proposer
---        let left_tree := @logarithmic_proposer _ mag _ sides_left prop_left
---        let right_tree := @logarithmic_proposer _ mag _ sides_right prop_right
---        match prop_mid
---              , get_total_range_tree left_tree
---              , get_total_range_tree right_tree
---        with
---        | .some (.Next p) , .some left_range, .some right_range =>
---          -- This is the mid condition that hashes meet here.
---          -- TODO Warning here
---          let h_mid := op_side sides_mid p.1 p.2
---          -- let h_mid := mag.comb p.1 p.2 -- I am not so sure about op_side
---          -- END TODO Warning here
---          -- But I need to get bounds from recursive calls.
---          let h_bot : ℍ := left_range.1
---          let h_top : ℍ := right_range.2
---          .node (.some ⟨(), ⟨ h_bot , h_mid ⟩, ⟨ h_mid , h_top ⟩⟩)
---                left_tree right_tree
---        | _ ,_ ,_ => .node .none left_tree right_tree
-----------------------------------------
-
-
--- Thm Winning proposer to winning proposer.
--- We have revealer/proposer winning conditions. I think we can prove through
--- that.
---
--- * Chooser is as bit complex.
--- Chooser needs to know the data to build a propoer chooser.
--- I am not sure we can define chooser transformation, same as we did with
--- proposer.
-----------------------------------------
-
--- Proposer wins all possible games.
--- leaf and mid winning conditions
--- @[simp]
-def elem_in_reveler_winning_condition {ℍ : Type}
-    [BEq ℍ][HashMagma ℍ]
-    {n : Nat}
-    (da : ElemInTreeH n ℍ)
-    (proposer : Sequence n (PMoves ℍ))
-    : Prop
     := match n with
-       | .zero => SingleLastStepH da = Player.Proposer
-       | .succ _pn =>
-         match headSeq proposer with
-         | .Next proposed =>
-           SingleMidStep  ⟨ da.mtree , proposed ⟩ = Player.Proposer
-           ∧ elem_in_reveler_winning_condition
-              (match headSeq da.data.2 with
-                | .inl _ =>
-                       ⟨ ⟨ da.data.1 , tailSeq da.data.2⟩ , proposed.1⟩
-                | .inr _ =>
-                       ⟨ ⟨ da.data.1 , tailSeq da.data.2⟩ , proposed.2⟩
-                )
-               (tailSeq proposer)
-
-----------------------------------------
--- DA + Proposer Algebra?
-
-def da_sum {ℍ : Type}{n m : Nat}
-  (da_l : ElemInTreeH n ℍ)
-  (da_r : ElemInTreeH m ℍ)
-  -- (_eq_bounds : da_l.mtree = da_r.data.1)
-  : ElemInTreeH (n + m) ℍ
-  := { data := ⟨ da_l.data.1 , concatSeq da_l.data.2 da_r.data.2 ⟩
-     , mtree := da_r.mtree}
-
-def da_split {ℍ : Type}{n : Nat}
-  -- Cut
-  ( m : Nat ) (mLtn : m ≤ n)
-  ( da : ElemInTreeH n ℍ )
-  ( mid : ℍ )
-  : ElemInTreeH m ℍ × ElemInTreeH (n - m) ℍ
-  := have ⟨ left , right ⟩ := splitSeq da.data.2 m mLtn
-  ⟨ {data := ⟨ da.data.1 , left ⟩ , mtree := mid }
-  , {data := ⟨ mid , right ⟩ , mtree := da.mtree } ⟩
-
-----------------------------------------
-
-----------------------------------------
--- * Alternative definition
--- Intermediary hashes with bounds
--- to_mid_step [0] = mtree
--- to_mid_step [last] = hash_botom
---
-def node_hashes { ℍ : Type }{n : Nat}
-    (da : ElemInTreeH n ℍ)
-    (proposer : Sequence n (PMoves ℍ))
-    : Sequence n.succ ℍ
-    := fun ⟨ m , mLt ⟩ =>
-    match HM : m with
-    | .zero => da.mtree -- good da when |n = 0|, da.data.1 = da.mtree
-    | .succ pm =>
-      match da.data.2 ⟨ pm , by omega⟩ , proposer ⟨ pm , by omega ⟩ with
-         | .inl _ , .Next proposed => proposed.1
-         | .inr _ , .Next proposed => proposed.2
-
-def logarithmic_proposer_hashes {ℍ}{lgn : Nat}
-    (da : ElemInTreeH (2^lgn.succ - 1 - 1) ℍ)
-    (proposer : Sequence (2^lgn.succ - 1 - 1) (PMoves ℍ))
-    : Sequence (2^lgn.succ - 1) ℍ
-    := sequence_coerce (by simp; have pZ := @pow_gt_zero lgn; omega )
-    $ node_hashes da proposer
-
-
-def complete_tree_proposer {ℍ : Type}{lgn : Nat}
-    (da : ElemInTreeH (2^lgn.succ - 1 - 1) ℍ)
-    (proposer : Sequence (2^lgn.succ - 1 - 1) (PMoves ℍ))
-    : ABTree ℍ ℍ
-    := perfectSeq $ logarithmic_proposer_hashes da proposer
-
-lemma complete_tree_decomp {ℍ : Type}{lgn : Nat}
-    -- At least two levels. One to use perfectSeq and another to put in mid.
-    (da : ElemInTreeH (2^lgn.succ.succ - 1 - 1 ) ℍ)
-    (proposer : Sequence (2^lgn.succ.succ -1 -1 ) (PMoves ℍ))
-    :
-    have ⟨ left, mid, right ⟩ := seqPerfectSplit (logarithmic_proposer_hashes da proposer)
-    perfectSeq (logarithmic_proposer_hashes da proposer)
-    = .node mid (perfectSeq left) (perfectSeq right)
-    := by
-      revert lgn
-      intro lgn
-      induction lgn with
-      | zero =>
-        intros da proposer
-        simp at *
-        simp [logarithmic_proposer_hashes, node_hashes, perfectSeq]
-      | succ pn HInd =>
-        intros da proposer
-        simp [seqPerfectSplit, splitSeq] -- left = takeN (2 ^ pn.succ.succ - 1) right = fail (dropN ..)
-
-
-
--- getters
-
-@[simp]
-def get_tree_distance {ℍ : Type} : ABTree (ℍ × Nat) (ℍ × Nat × ℍ × Nat × ℍ ) -> Nat
-  := ABTree.getI' (fun p => p.2) (fun p=> p.2.1 + p.2.2.2.1)
-
-def get_bot_hash {ℍ : Type} : ABTree (ℍ × Nat) (ℍ × Nat × ℍ × Nat × ℍ ) -> ℍ
- := ABTree.getI' (fun p => p.1) (fun p => p.1)
-def get_top_hash {ℍ : Type} : ABTree (ℍ × Nat) (ℍ × Nat × ℍ × Nat × ℍ ) -> ℍ
- := ABTree.getI' (fun p => p.1) (fun p => p.2.2.2.2)
-
-def tree_distance {ℍ : Type} : ABTree ℍ ℍ -> ABTree (ℍ × Nat) (ℍ × Nat × ℍ × Nat × ℍ )
-  | .leaf b => .leaf ⟨ b, 0 ⟩
-  | .node h (.leaf l) (.leaf r) =>
-    .node ⟨ l , 1 , h , 1, r ⟩
-          (.leaf ⟨ l, 0 ⟩) (.leaf ⟨r , 0 ⟩)
-  | .node h (.leaf l) b =>
-    let b' := tree_distance b
-    .node ⟨ l , 1 , h , get_tree_distance b' , get_top_hash b'⟩
-          (.leaf ⟨ l , 0 ⟩) b'
-  | .node h b (.leaf r) =>
-    let b' := tree_distance b
-    .node ⟨ get_bot_hash b', get_tree_distance b' , h , 1, r ⟩
-          b' (.leaf ⟨ r , 0 ⟩)
-  | .node h bl br =>
-      let bl' := tree_distance bl
-      let br' := tree_distance br
-      .node ⟨ get_bot_hash bl'
-            , get_tree_distance bl'
-            , h
-            , get_tree_distance br'
-            , get_bot_hash br'
-            ⟩
-        bl' br'
-
-def da_generator {ℍ : Type}
-  (info : ℍ × Nat × ℍ × Nat × ℍ )
-  : DA_Statement ℍ × DA_Statement ℍ
-  := ⟨ {src := info.1, dst := info.2.2.1, len := info.2.1}
-     , {src := info.2.2.1, dst := info.2.2.2.2, len := info.2.2.2.1} ⟩
-
-def tree_da_generator {ℍ : Type}
-  : ABTree ℍ  ℍ
-  -> ABTree ℍ (DA_Statement ℍ × DA_Statement ℍ)
-  := ABTree.map (fun p => p.1) da_generator
-     ∘ tree_distance
-
-----------------------------------------
-
--- We are defining the same lemmas and theorems as the first implementations.
-theorem forall_mid_step {ℍ : Type}
-    [BEq ℍ][HashMagma ℍ] {n : Nat}
-    (da : ElemInTreeH n ℍ)
-    (proposer : Sequence n (PMoves ℍ))
-    (winning_cond : elem_in_reveler_winning_condition da proposer)
-    :
-    forall (i : Nat)(iNZ : 0 < i)(iLtn : i < n),
-        SingleMidStep ⟨ node_hashes da proposer ⟨ i , by omega ⟩
-                      , (proposer ⟨ i , iLtn ⟩).destruct
-                      ⟩ = Player.Proposer
-    := sorry
-
-theorem last_hash_node_hashes {ℍ : Type}
-    [BEq ℍ][HashMagma ℍ] {n : Nat}
-    (da : ElemInTreeH n ℍ)
-    (proposer : Sequence n (PMoves ℍ))
-    (winning_cond : elem_in_reveler_winning_condition da proposer)
-    : da.data.1 =  lastSeq (node_hashes da proposer)
-    := sorry
-
-theorem first_hash_node_hashes {ℍ : Type}
-    [BEq ℍ][HashMagma ℍ] {n : Nat}
-    (da : ElemInTreeH n ℍ)
-    (proposer : Sequence n (PMoves ℍ))
-    (winning_cond : elem_in_reveler_winning_condition da proposer)
-    : da.mtree = headSeq (node_hashes da proposer)
-    := sorry
-
--- This are the winning conditions, I first proposed long time ago.
--- So we already have a logarithmic proposer definition and a winning condition.
-
-
-theorem winning_reveler_sum {ℍ : Type}
-    [BEq ℍ][LawfulBEq ℍ][HashMagma ℍ]
-    {n m : Nat}
-    -- Revelers
-    (da_l : ElemInTreeH n ℍ)(proposer_l : Sequence n (PMoves ℍ))
-    (good_left : elem_in_reveler_winning_condition da_l proposer_l)
-    (da_r : ElemInTreeH m ℍ)(proposer_r : Sequence m (PMoves ℍ))
-    (good_right : elem_in_reveler_winning_condition da_r proposer_r)
-    -- Such that share a meeting point
-    (eq_mid : da_l.mtree = da_r.data.1)
-    : elem_in_reveler_winning_condition (da_sum da_l da_r)
-                                        (concatSeq proposer_l proposer_r)
-    := by unfold elem_in_reveler_winning_condition
-          revert m
-          intro m
-          induction m with
-          | zero =>
-            intros da_r proposer_r good_right eq_mid
-            simp
-            cases n with
-            | zero =>
-              simp [SingleLastStepH, condWProp,da_sum];
-              unfold elem_in_reveler_winning_condition at good_right
-              simp [SingleLastStepH, condWProp] at good_right
-              unfold elem_in_reveler_winning_condition at good_left
-              simp [SingleLastStepH, condWProp] at good_left;
-              rwa [good_left,eq_mid]
-            | succ pn =>
-              simp [da_sum]
-              unfold elem_in_reveler_winning_condition at good_left
-              cases H : headSeq proposer_l with
-              -- | none => rw [H] at good_left; simp at good_left
-              | Next proposed =>
-                rw [H] at good_left; simp at good_left
-                -- replace (.Next proposed) := proposed
-                simp at H; rw [H]; simp
-                sorry
-              | End a => contradiction
-          | succ pm HInd =>
-                 sorry
-
--- We can split das, but we need a ℍ to split it.
-def split_da {ℍ}{n : Nat}
-    (da : ElemInTreeH n ℍ)
-    (cut_h : ℍ)
-    (m : Nat)( mLtn : m ≤ n) -- 0 < n
-    : (ElemInTreeH m ℍ × ElemInTreeH (n - m) ℍ)
-    := let ⟨ left_skl , right_skl ⟩ := splitSeq da.data.2 m mLtn
-      ⟨ {data := ⟨ da.data.1 , left_skl⟩ , mtree := cut_h}
-      , {data := ⟨ cut_h , right_skl⟩ , mtree := da.mtree} ⟩
-
--- General cuttings
-theorem split_da_concatSeq {ℍ}[BEq ℍ][HashMagma ℍ]{n : Nat}
-  (da : ElemInTreeH n ℍ)
-  (rev : Sequence n (PMoves ℍ))
-  --
-  (lin_rev : elem_in_reveler_winning_condition da rev)
-  --
-  (cut : Nat)(cutLtn : cut < n)
-  : let .Next p := (rev ⟨ cut , by omega ⟩)
-    let ⟨ da_left, _ ⟩ :=
-      split_da da (match da.data.2 ⟨ cut , by omega ⟩ with
-         | .inl _ => p.1
-         | .inr _ => p.2) cut (by omega)
-    elem_in_reveler_winning_condition da_left (splitSeq rev cut (by omega)).1
-  := sorry
-
--- Perfect Splitting DAs  + Reveler + Winning conditions
-theorem split_da_perfect_left {ℍ}[BEq ℍ][HashMagma ℍ]{lgn : Nat}
-  (da : ElemInTreeH (2^lgn.succ - 1) ℍ)
-  (rev : Sequence (2^lgn.succ - 1) (PMoves ℍ))
-  -- Good rev
-  (lin_rev : elem_in_reveler_winning_condition da rev)
-  : let ⟨ left_skl, mid_skl, right_skl ⟩ := seqPerfectSplit da.data.2
-    let ⟨ left_rev, mid_rev, right_rev ⟩ := seqPerfectSplit rev
-    let ⟨ h_rev_l , h_rev_r ⟩ := mid_rev.destruct
-    let top_hash := match mid_skl with
-                          | .inl _ => h_rev_l
-                          | .inr _ => h_rev_r
-    let da_left := {data := ⟨ da.data.1 , left_skl ⟩, mtree := top_hash}
-    elem_in_reveler_winning_condition da_left left_rev
-  := sorry
-
-theorem split_da_perfect_right {ℍ}[BEq ℍ][HashMagma ℍ]{lgn : Nat}
-  (da : ElemInTreeH (2^lgn.succ - 1) ℍ)
-  (rev : Sequence (2^lgn.succ - 1) (PMoves ℍ))
-  -- Good rev
-  (lin_rev : elem_in_reveler_winning_condition da rev)
-  : let ⟨ left_skl, mid_skl, right_skl ⟩ := seqPerfectSplit da.data.2
-    let ⟨ left_rev, mid_rev, right_rev ⟩ := seqPerfectSplit rev
-    let ⟨ h_rev_l , h_rev_r ⟩ := mid_rev.destruct
-    let bot_hash := match mid_skl with
-                          | .inl _ => h_rev_l
-                          | .inr _ => h_rev_r
-    --
-    let da_right := { data  := ⟨ op_side mid_skl h_rev_l h_rev_r, right_skl ⟩
-                    , mtree := da.mtree}
-    elem_in_reveler_winning_condition da_right right_rev
-  := sorry
-----------------------------------------
-
-@[simp]
-def log_winning_game {ℍ : Type}
-    [BEq ℍ][HashMagma ℍ]
-    (da : Tree_DA ℍ)
-    -- Players
-    (reveler : Tree_Reveler ℍ)
-    : Prop
-    := reveler_winning_condition
-        leaf_condition_transformation
-        mid_condition_transformation
-        da reveler
-
-def gen_tree {ℍ : Type}(height : Nat)(l r : ℍ)
-  : Tree_DA ℍ
-  := { data := gen_empty_perfect_tree height
-     , res := ⟨ l, r , (2^height.succ - 1 - 1) ⟩ }
-
--- def da_to_tree {ℍ : Type}{lgn : Nat}
---     (da : ElemInTreeH (2^lgn.succ - 1) ℍ)
---     : Tree_DA ℍ
---     := { data := perfectSeq $ seqMap (fun _ => ()) da.data.2
---        , res  := ⟨ da.data.1 , da.mtree ⟩}
-
--- def tree_composition {ℍ : Type}
---     [BEq ℍ][LawfulBEq ℍ][mag : HashMagma ℍ]
---     --
---     (left_da  : Tree_DA ℍ)
---     (left_rev : Tree_Reveler ℍ)
---     --
---     (right_da  : Tree_DA ℍ)
---     (right_rev : Tree_Reveler ℍ)
---     -- Stuff
---     : Tree_DA ℍ × Tree_Reveler ℍ :=
---     let h_mid := mag.comb <$> left_rev.top <*> right_rev.top
---     ⟨{ data := .node () left_da.data right_da.data
---       , res := ⟨ left_da.res.1 , right_da.res.2⟩} -- [a , b]
---     , .node ( h_mid.map (fun h => ⟨ ()
---                                   , ⟨left_da.res.1 , h⟩ -- [a, mid]
---                                   , ⟨h , right_da.res.2⟩ ⟩)) -- [mid , b]
---             left_rev right_rev ⟩
-
--- theorem tree_composition_winning {ℍ : Type}
-      -- log_winning_game
-      --    {data := .node _ _ _
-      --    , res := ⟨ left_da.data.1 , right_da.mtree ⟩}
-      --    (.node (.some ( ⟨ () , ⟨left_da.data.1 , h_mid⟩ , ⟨ h_mid ,right_da.mtree ⟩ ⟩))
-      --                  (@logarithmic_proposer _ mag _ left_da.data.2
-      --                                                  (seqMap .some left_rev))
-      --                  (@logarithmic_proposer _ mag _ right_da.data.2
-      --                                     (seqMap .some right_rev))
-      --    )
-
-
-theorem linear_to_log_winning_proposer {ℍ : Type}
-    [BEq ℍ][LawfulBEq ℍ][mag : HashMagma ℍ]
-    -- DA
-    {lgn : Nat}
-    (da : ElemInTreeH (2^lgn.succ - 1 - 1) ℍ)
-    -- Reveler
-    (lin_reveler : Sequence (2^lgn.succ - 1 - 1) (PMoves ℍ))
-    (win_lin : elem_in_reveler_winning_condition da lin_reveler)
-    : reveler_winning_condition
-        leaf_condition_transformation
-        mid_condition_transformation
-        -- DA is just a tree generate of height lgn and
-        -- boundaries [da.data.1, da.mtree]
-        (gen_tree lgn da.data.1 da.mtree)
-        --
-        (( tree_da_generator (complete_tree_proposer da lin_reveler) ).map .some (fun p => .some ⟨ (), p⟩))
-    := by
-    revert lgn
-    intro lgn
-    induction lgn with
-    | zero =>
-      intros da lin_rev HElem
-      simp [complete_tree_proposer,perfectSeq,logarithmic_proposer_hashes, tree_da_generator]
-      simp [tree_distance]
-      simp [node_hashes]
-      simp [gen_tree]
-      simp [gen_empty_perfect_tree,reveler_winning_condition]
-      simp [leaf_condition_transformation]
-      simp [condWProp]
-      unfold elem_in_reveler_winning_condition at HElem
-      simp [SingleLastStepH,condWProp] at HElem
-      constructor
-      rw [HElem]
-      assumption
-    | succ plgn HInd =>
-      intros da lin_rev HElem
-
-      simp [complete_tree_proposer,logarithmic_proposer_hashes, perfectSeq, tree_da_generator]
-      simp [seqPerfectSplit, splitSeq]
+      | 0 => SingleLastStepH da
+      | .succ _pn =>
+        match lastSeq proposer with
+        | .none => Player.Chooser
+        | .some (.Next proposed) =>
+            match lastSeq chooser ⟨ da.mtree.1, proposed ⟩ with
+            | .none  => Player.Proposer
+            | .some .Now =>
+              forward_mid_step_condition
+                (lastSeq da.data) ⟨ da.mtree.1 , proposed.2⟩ proposed.1
+            | .some (.Continue _) =>
+              elem_in_tree_forward
+                {data := Fin.init da.data, mtree := ⟨ proposed.1 , da.mtree.2⟩}
+                (Fin.init proposer)
+                (Fin.init chooser)
