FraudProof/Games/Base/PathToTreeGames.lean
@@ -1,0 +1,234 @@
+import FraudProof.Games.GameDef -- Players, Winner
+import FraudProof.Games.Base.GenericTree -- Generic Game trees
+import FraudProof.Games.Base.ElemInTree -- Linear basic game definition
+import FraudProof.Games.Base.RangeDAConditions -- Range DAs
+
+import FraudProof.DataStructures.Sequence
+
+--------------------------------------------------------------------------------
+-- * Transformation from a Sequence to the /same/ game played over Trees arenas.
+--------------------------------------------------------------------------------
+
+-- Building a Tree out of skelentons.
+-- This function keeps size.
+-- ABTree.size is height
+@[simp]
+def skl_to_tree {n : Nat}
+  (sk : ISkeleton n) : ABTree Unit Unit
+  := match n with
+    | .zero => .leaf ()
+    | .succ _pn =>
+      match headSeq sk with
+        | .inl _ => .node () (skl_to_tree $ Fin.tail sk) (.leaf ())
+        | .inr _ => .node () (.leaf ()) (skl_to_tree $ Fin.tail sk)
+@[simp]
+def skl_to_maybe_elem {α : Type} {n : Nat}
+  (a : α) (sk : ISkeleton n) : ABTree (Option α) Unit
+    := match n with
+    | .zero => .leaf a
+    | .succ _pn =>
+      match headSeq sk with
+        | .inl _ =>
+          .node () (skl_to_maybe_elem a (Fin.tail sk)) (.leaf none)
+        | .inr _ =>
+          .node () (.leaf none) (skl_to_maybe_elem a (Fin.tail sk))
+
+
+@[simp]
+def build_proposer' {ℍ : Type}{n : Nat}
+    (bot_hash : ℍ)
+    (skl : ISkeleton n)
+    (rev : Sequence n (Option (PMoves ℍ)))
+    : ABTree (Option ℍ) (Option (SkElem × Range ℍ × Range ℍ))
+    := match n with
+    | .zero => .leaf $ .some bot_hash
+    | .succ _ =>
+      match headSeq rev with
+      | .none => .node .none (.leaf none) (.leaf none)
+      | .some (.Next proposed) =>
+        match headSeq skl with
+        | .inl _ =>
+               .node (.some ( ⟨ .inl () , ⟨ bot_hash , proposed.1⟩ , proposed  ⟩ ))
+                     (build_proposer' bot_hash (Fin.tail skl) (Fin.tail rev))
+                     (.leaf $ .some proposed.2)
+        | .inr _ =>
+               .node (.some ( ⟨ .inr () , ⟨ bot_hash , proposed.2 ⟩ , proposed  ⟩ ))
+                     (build_proposer' bot_hash (Fin.tail skl) (Fin.tail rev))
+                     (.leaf $ .some proposed.1)
+
+@[simp]
+def build_proposer {ℍ : Type}{n : Nat}
+  (data : ℍ × ISkeleton n) (rev : Sequence n (Option (PMoves ℍ)))
+  : ABTree (Option ℍ) (Option (Unit × ℍ × ℍ))
+  := match n with
+  | .zero => .leaf $ .some data.1
+  | .succ _pn =>
+    let rest_tree := build_proposer ⟨ data.1 , Fin.tail data.2⟩ (Fin.tail rev)
+    match headSeq rev with
+      | .none => .node .none (.leaf none) (.leaf .none)
+      | .some (.Next ⟨ hl , hr⟩)=>
+       match headSeq data.2 with
+         | .inl _ =>
+           .node (.some ⟨ (), hl, hr ⟩)
+                 rest_tree
+                 (.leaf (.some hr))
+         | .inr _ =>
+           .node (.some ⟨ (), hl, hr ⟩)
+                 (.leaf (.some hl))
+                 rest_tree
+@[simp]
+def build_chooser {ℍ : Type}{n : Nat}
+  (data : ℍ × ISkeleton n)
+  (chooser : Sequence n (ℍ × ℍ × ℍ -> Option ChooserSmp))
+  : ABTree Unit (ℍ × Unit × ℍ × ℍ -> Option ChooserMoves)
+  := match n with
+    | .zero => .leaf ()
+    | .succ _pn =>
+      let side_choose (s : Chooser.Side) (arg : ℍ × Unit × ℍ × ℍ)
+          : Option ChooserMoves :=
+          have ⟨ ht , _ , hl , hr ⟩ := arg
+          (headSeq chooser ⟨ ht, hl , hr ⟩).map
+            (fun ch => match ch with
+                       | .Now => .Now
+                       | .Continue _ => .Continue s)
+      match headSeq data.2 with
+      | .inl _ =>
+        .node
+          (side_choose .Left)
+          (build_chooser ⟨data.1 , Fin.tail data.2⟩ (Fin.tail chooser))
+          (.leaf ())
+      | .inr _ =>
+        .node
+          (side_choose .Right)
+          (.leaf ())
+          (build_chooser ⟨data.1 , Fin.tail data.2⟩ (Fin.tail chooser))
+
+@[simp]
+def build_chooser' {ℍ : Type}{n : Nat}
+  (skl : ISkeleton n)
+  (chooser : Sequence n (ℍ × ℍ × ℍ -> Option ChooserSmp))
+  : ABTree Unit (Range ℍ × SkElem  × Range ℍ × Range ℍ -> Option ChooserMoves)
+  := match n with
+    | .zero => .leaf ()
+    | .succ _ =>
+      let curr_check (args : Range ℍ × SkElem  × Range ℍ × Range ℍ)
+                     : Option ChooserMoves
+        := -- Should I check Range consistency? Not necesseary during transformations
+          have ⟨ top_range, side, _next_range, decomp ⟩ := args
+          -- top_range.1 == next_range.1 && next_range.2 == decomp.side
+          match side with
+          | .inl _ => match headSeq chooser ⟨ top_range.2, decomp.1, decomp.2 ⟩ with
+                      | .some .Now => .some .Now
+                      | .some (.Continue _) => .some $ .Continue .Left
+                      | .none => .none
+          | .inr _ => match headSeq chooser ⟨ top_range.2, decomp.2, decomp.1 ⟩ with
+                      | .some .Now => .some .Now
+                      | .some (.Continue _) => .some $ .Continue .Right
+                      | .none => .none
+      match headSeq skl with
+      | .inl _ => .node curr_check (build_chooser' (Fin.tail skl) (Fin.tail chooser)) (.leaf ())
+      | .inr _ => .node curr_check (.leaf ()) (build_chooser' (Fin.tail skl) (Fin.tail chooser))
+
+
+def elem_in_tree_gen_tree {ℍ : Type}
+    [BEq ℍ][mag : HashMagma ℍ]
+    -- DA
+    {n : Nat}
+    (da : ElemInTreeH n ℍ)
+    --
+    (proposer : Sequence n (Option (PMoves ℍ)))
+    (chooser : Sequence n (ℍ × ℍ × ℍ -> Option ChooserSmp))
+    --
+    : Winner
+    :=
+    let da_tree : CompTree (Option ℍ) Unit ℍ
+      := {data := skl_to_maybe_elem da.mtree.1 da.data , res := da.mtree.2}
+    let tree_revealer : ABTree (Option ℍ) (Option (Unit × ℍ × ℍ))
+      := build_proposer ⟨ da.mtree.1 , da.data⟩ proposer
+    let tree_chooser : ABTree Unit (ℍ × Unit × ℍ × ℍ -> Option ChooserMoves)
+      := build_chooser ⟨ da.mtree.1 , da.data⟩ chooser
+    treeCompArbGame
+      (fun opth _h1 h2 =>
+        match opth with
+        | .none => -- this case is a bit artificial
+        -- chooser should challenge previous step.
+          Player.Proposer
+        | .some hp => condWProp <| (hp == h2)
+      )
+      (fun _ _ hres pl pr =>
+        -- _nodeh and hres should be the same.
+           condWProp $ mag.comb pl pr == hres)
+      da_tree tree_revealer tree_chooser
+
+def elem_in_tree_forward_gentree {ℍ : Type}
+    [BEq ℍ][mag : HashMagma ℍ]
+    -- DA
+    {n : Nat}(da : ElemInTreeH n ℍ)
+    -- Players
+    (proposer : Sequence n (Option (PMoves ℍ)))
+    (chooser : Sequence n (ℍ × ℍ × ℍ -> Option ChooserSmp))
+    :=
+    treeCompArbGame
+      -- conditionsb
+      leaf_condition_range
+      mid_condition_range_one_step_forward
+      -- DA
+      {data := skl_to_tree da.data, res:= da.mtree}
+      (build_proposer' da.mtree.1 da.data proposer)
+      (build_chooser' da.data chooser)
+----------------------------------------
+-- Are both games equivs?
+--
+--Two games (in this case) are equivalente if they have the same outcome to the
+--same players.
+
+theorem seq_equiv_tree {ℍ : Type}[BEq ℍ][HashMagma ℍ]
+  -- DA
+  {n : Nat}(da : ElemInTreeH n ℍ)
+  -- Players
+  (proposer : Sequence n (Option (PMoves ℍ)))
+  (chooser : Sequence n (ℍ × ℍ × ℍ -> Option ChooserSmp))
+  : elem_in_tree_backward da proposer chooser = elem_in_tree_gen_tree da proposer chooser
+  := by revert n
+        intro n
+        induction n with
+        | zero =>
+          intros da prop cho
+          simp [elem_in_tree_backward, elem_in_tree_gen_tree, SingleLastStepH, treeCompArbGame]
+        | succ pn HInd =>
+          intros da prop cho
+          simp [elem_in_tree_backward, elem_in_tree_gen_tree ]
+          cases prop 0 with
+          | none =>
+            simp [treeCompArbGame]
+          | some proposed =>
+            cases proposed with
+            | End v => contradiction
+            | Next e =>
+              simp
+              match HCho : cho 0 (da.mtree.2, e) with
+              | none =>
+                simp [treeCompArbGame]
+                match da.data 0 with
+                | .inl _ => simp [treeCompArbGame]; rw [HCho]; simp
+                | .inr _ => simp [treeCompArbGame]; rw [HCho]; simp
+              | some choosed =>
+                match choosed with
+                | .Now =>
+                  simp [SingleMidStep]
+                  cases da.data 0 with
+                    | inl _ => simp [treeCompArbGame]; rw [HCho]; simp
+                    | inr _ => simp [treeCompArbGame]; rw [HCho]; simp
+                | .Continue _ =>
+                  simp
+                  cases da.data 0 with
+                    | inl _ =>
+                      simp [treeCompArbGame]
+                      rw [HCho]; simp
+                      apply HInd
+                    | inr _ =>
+                      simp [treeCompArbGame]
+                      rw [HCho]; simp
+                      apply HInd
+
+----------------------------------------
